pulse/ulib/experimental/Steel.Effect.Atomic.fst
@@ -21,6 +21,8 @@ open Steel.EffectX.Atomic
 friend Steel.EffectX.Atomic
 friend Steel.Effect
 
+#set-options "--warn_error -330"  //turn off the experimental feature warning
+
 let observability = observability
 let has_eq_observability = has_eq_observability
 let observable = observable
